Max Eliminator verified

theories/Compositional_Structures/Basic_Modules/Component_Types/Elimination_Module_Ref.thy
@@ -16,10 +16,6 @@ text \<open>
 
 subsection \<open>Definition\<close>
 
-type_synonym Threshold_Value = "nat"
-
-type_synonym Threshold_Relation = "nat \<Rightarrow> nat \<Rightarrow> bool"
-
 type_synonym 'a Scores_Map = "('a \<rightharpoonup> nat)"
 
 definition pre_compute_scores :: "'a Evaluation_Function_Ref \<Rightarrow>
@@ -44,8 +40,6 @@ definition scoremax :: "'a set \<Rightarrow> 'a Scores_Map \<Rightarrow> nat nre
     }) (0::nat)
 }"
 
-
-
 definition eliminate:: "'a Scores_Map  \<Rightarrow> Threshold_Value \<Rightarrow>
                             Threshold_Relation \<Rightarrow> 
                           'a set \<Rightarrow> 'a Profile_List \<Rightarrow> ('a set \<times> 'a set) nres" where
@@ -59,9 +53,9 @@ definition eliminate:: "'a Scores_Map  \<Rightarrow> Threshold_Value \<Rightarro
       else 
           RETURN(rej, insert x def))
     }) ({}, {})
-
-    
 }"
+
+
 
 definition elimination_module_ref :: 
 "'a Scores_Map  \<Rightarrow> Threshold_Value \<Rightarrow>
@@ -71,7 +65,7 @@ Threshold_Relation \<Rightarrow> 'a Electoral_Module_Ref "
     (rej, def) <- eliminate scores threshold r A p;
    if (def = {}) then
        \<comment> \<open>Here rej will be a copy of A\<close>
-     RETURN({},{},rej)
+     RETURN ({},{},rej)
     else
      RETURN ({},rej,def)
   }"
@@ -80,8 +74,70 @@ Threshold_Relation \<Rightarrow> 'a Electoral_Module_Ref "
 definition pre_computed_map :: "'a Evaluation_Function \<Rightarrow> 'a set \<Rightarrow> 'a Profile \<Rightarrow> ('a \<rightharpoonup> nat)"  where
   "pre_computed_map e Alts pro \<equiv> ((\<lambda>a. Some (e a Alts pro))|`Alts )"
 
+
+lemma eliminate_correct:
+  fixes e :: "'a Evaluation_Function"
+  and A :: "'a set"
+  and t :: "Threshold_Value"
+  and r :: "Threshold_Relation"
+  assumes fina: "finite A"
+  shows "(eliminate (pre_computed_map e A pr) t r A pl \<le> 
+    SPEC (\<lambda> (rej,def). (rej,def) = ((elimination_set e t r A pr), A - (elimination_set e t r A pr))))"
+  unfolding pre_computed_map_def eliminate_def
+  apply (refine_vcg FOREACH_rule
+      [where I = "\<lambda> it (rej, def). rej = ((elimination_set e t r A pr) - it)
+                \<and> def = (A - it) - (elimination_set e t r (A) pr)"])
+  by (auto simp add: fina)
+
+
 context voting_session
 begin
+
+theorem elimination_module_ref_correct:
+  fixes efn :: "'a Evaluation_Function"
+  and t :: "Threshold_Value"
+  and r :: "Threshold_Relation"
+  shows "(elimination_module_ref (pre_computed_map efn A pr) t r A pl \<le> 
+            SPEC (\<lambda> em. em = (elimination_module efn t r A pr)))"
+  unfolding  elimination_module_ref_def
+  apply (refine_vcg eliminate_correct)
+  by (auto simp add: fina)
+
+lemma compute_scores_correct_weak_evalref:
+  fixes eref :: "'a Evaluation_Function_Ref"
+  and e :: "'a Evaluation_Function"
+  assumes "((\<lambda> x. eref x A), (\<lambda> x p. RETURN ( e x A p))) \<in> evalf_profA_rel A"
+  shows "(pre_compute_scores eref A pl, SPEC (\<lambda> map. map = pre_computed_map e A pr)) \<in> 
+    \<langle>Id\<rangle>nres_rel"
+  unfolding pre_compute_scores_def pre_computed_map_def
+  apply (refine_vcg FOREACH_rule[where I = 
+        "(\<lambda>it r. r = (\<lambda> a. Some (e a A pr))|`(A - it))"])
+  apply (auto simp add: fina)
+proof -
+  fix x:: 'a
+  fix it:: "'a set"
+  assume xit: "x \<in> it"
+  assume itA: "it \<subseteq> A"
+  from xit itA have xiA: "x \<in> A" by fastforce
+  from xit itA have wcr: "((\<lambda>a. Some (e a A pr)) |` (A - it))(x \<mapsto> (e x A pr)) =
+                      (\<lambda>a. Some (e a A pr)) |` (A - (it - {x}))"
+      using it_step_insert_iff restrict_map_insert
+      by metis
+  from this have mapupdeq: "(\<lambda>scx. ((\<lambda>a. Some (e a A pr)) |` (A - it))(x \<mapsto> scx) =
+                   (\<lambda>a. Some (e a A pr)) |` (A - (it - {x})))
+      = (\<lambda> wc. wc = (e x A pr))"
+    by (metis map_upd_eqD1)
+  from profrel have prel: "(pl, pr) \<in> profile_rel" using profile_type_ref by auto
+  from profrel assms(1)[THEN fun_relD, THEN fun_relD, THEN nres_relD]
+    this have "(eref x A pl) \<le> SPEC(\<lambda> scx. scx = (e x A pr))"
+    by (metis IdI SPEC_eq_is_RETURN(2) refine_IdD) 
+  from this mapupdeq show " (eref x A pl)
+       \<le> SPEC (\<lambda>scx. ((\<lambda>a. Some (e a A pr)) |` (A - it))(x \<mapsto> scx) =
+                      (\<lambda>a. Some (e a A pr)) |` (A - (it - {x})))"
+    using SPEC_cons_rule it_step_insert_iff restrict_map_insert
+    by presburger 
+qed 
+
 
 lemma compute_scores_correct:
   fixes eref :: "'a Evaluation_Function_Ref"
@@ -119,8 +175,6 @@ proof -
 qed 
 
 lemma scoremax_correct:
-  fixes e :: "'a Evaluation_Function"
-  assumes "(eref, (\<lambda> a Alts pro. RETURN (e a Alts pro))) \<in> evalf_rel"
   shows "scoremax A (pre_computed_map e A pr) 
 \<le> SPEC (\<lambda> max. max = Max {(e a A pr) | a. a \<in> A})"
   unfolding scoremax_def pre_computed_map_def
@@ -149,7 +203,7 @@ subsection \<open>Common Eliminators\<close>
                                    
 fun less_eliminator_ref :: "'a Scores_Map  \<Rightarrow> Threshold_Value \<Rightarrow>
                             'a Electoral_Module_Ref" where
-  "less_eliminator_ref e tc A p = elimination_module_ref e tc (<) A p"
+  "less_eliminator_ref e t A p = elimination_module_ref e t (<) A p"
 
 fun max_eliminator_ref ::  "'a Scores_Map \<Rightarrow>
                             'a Electoral_Module_Ref" where
@@ -157,6 +211,27 @@ fun max_eliminator_ref ::  "'a Scores_Map \<Rightarrow>
     t <- (scoremax A e); 
     (less_eliminator_ref e t A p)
  }"
+
+context voting_session
+begin
+
+lemma less_eliminator_correct:
+  fixes efn :: "'a Evaluation_Function"
+  and t :: "Threshold_Value"
+  shows "(less_eliminator_ref (pre_computed_map efn A pr) t A pl \<le>
+            SPEC (\<lambda> em. em = (less_eliminator efn t A pr)))"
+  unfolding less_eliminator_ref.simps less_eliminator.simps
+  by (refine_vcg elimination_module_ref_correct)
+
+theorem max_eliminator_ref_correct:
+  fixes efn :: "'a Evaluation_Function"
+  shows "(max_eliminator_ref (pre_computed_map efn A pr) A pl \<le>
+            SPEC (\<lambda> em. em = max_eliminator efn A pr))"
+  unfolding max_eliminator_ref.simps max_eliminator.simps
+  apply (refine_vcg scoremax_correct less_eliminator_correct)
+  by auto
+
+end
 
 fun leq_eliminator_ref :: "'a Scores_Map \<Rightarrow> Threshold_Value \<Rightarrow>
                             'a Electoral_Module_Ref" where
