theories/Compositional_Structures/Basic_Modules/Component_Types/Evaluation_Function_Ref.thy
@@ -23,9 +23,10 @@ subsection \<open>Definition\<close>
 
 type_synonym 'a Evaluation_Function_Ref = "'a  \<Rightarrow> 'a set \<Rightarrow> 'a Profile_List \<Rightarrow> nat nres"
 
-
-
 abbreviation "evalf_rel \<equiv> Id \<rightarrow> \<langle>Id\<rangle>set_rel \<rightarrow> profile_rel \<rightarrow> \<langle>nat_rel\<rangle>nres_rel"
+
+abbreviation "evalf_profA_rel A \<equiv> Id \<rightarrow> profile_on_A_rel A \<rightarrow> \<langle>nat_rel\<rangle>nres_rel"
+
 
 lemma evalfeq:   
   fixes A:: "'a set" 
